Replace Ne predicate by self-convertibility at neutral.

theories/LogicalRelation/Neutral.v
@@ -7,14 +7,13 @@ Set Universe Polymorphism.
 Section Neutral.
 Context `{GenericTypingProperties}.
 
-Definition neu {l Γ A} : Ne[Γ |- A] -> [Γ |- A] -> [ Γ |- A ~ A : U] -> [Γ ||-<l> A].
+Definition neu {l Γ A} : [Γ |- A] -> [ Γ |- A ~ A : U] -> [Γ ||-<l> A].
 Proof.
-  intros neA wtyA reflA. apply LRne_.
+  intros wtyA reflA. apply LRne_.
   exists A; [gen_typing|..]; assumption.
 Defined.
 
 Lemma neU {l Γ A n} (h : [Γ ||-U<l> A]) :
-  Ne[Γ |- n : A] ->
   [Γ |- n : A] ->
   [Γ |- n ~ n : A] ->
   [LogRelRec l | Γ ||-U n : A | h].
@@ -22,12 +21,10 @@ Proof.
   assert [Γ |- A ≅ U] by (destruct h; gen_typing).
   intros; exists n.
   * eapply redtmwf_conv; tea; now eapply redtmwf_refl.
-  * now eapply NeType, tm_ne_whne.
-  * eapply tm_nf_conv; [|gen_typing|eassumption].
-    now eapply tm_ne_nf.
-  * eapply convtm_conv; tea; gen_typing.
-  * eapply RedTyRecBwd, neu. 2,3: gen_typing.
-    eapply ty_ne_term, tm_ne_conv; now gen_typing.
+  * now eapply NeType, convneu_whne.
+  * eapply convtm_conv; [|tea].
+    now apply convtm_convneu.
+  * eapply RedTyRecBwd, neu. 1,2: gen_typing.
 Defined.
 
 
@@ -55,12 +52,11 @@ Set Printing Primitive Projection Parameters.
 
 
 Lemma neuEq {l Γ A B} (RA : [Γ ||-<l> A]) :
-  Ne[Γ |- A] -> Ne[Γ |- B] ->
   [Γ |- A] -> [Γ |- B] ->
   [Γ |- A ~ B : U] ->
   [Γ ||-<l> A ≅ B | RA].
 Proof.
-  intros neA neB wtyA wtyB eqAB.
+  intros wtyA wtyB eqAB.
   unshelve irrelevance0. 1: assumption. 3: reflexivity.
   1: apply neu; try assumption; now eapply lrefl.
   econstructor.
@@ -91,38 +87,19 @@ Proof.
   gen_typing.
 Qed.
 
-Lemma neu_app_ren {Γ Δ A n a dom cod} (ρ : Δ ≤ Γ) :
-  [|- Δ] ->
-  [Γ |- tProd dom cod] ->
-  Ne[Γ |- n : A] -> [Γ |- A ≅ tProd dom cod] -> Nf[Δ |- a : dom⟨ρ⟩] -> Ne[Δ |- tApp n⟨ρ⟩ a : cod[a .: ρ >> tRel]].
-Proof.
-  intros.
-  replace (cod[a .: ρ >> tRel]) with (cod⟨wk_up dom ρ⟩[a..]) by (now bsimpl).
-  eapply tm_ne_app; [|eassumption].
-  change (Ne[Δ |- n⟨ρ⟩ : (tProd dom cod)⟨ρ⟩]).
-  eapply tm_ne_conv; [| |now eapply convty_wk].
-  + now eapply tm_ne_wk.
-  + now eapply wft_wk.
-Qed.
-
 Record complete {l Γ A} (RA : [Γ ||-<l> A]) := {
-  reifyTyConv : forall B, [Γ ||-<l> A ≅ B | RA] -> Nf[Γ |- B];
   reflect : forall n n',
-    Ne[Γ |- n : A] ->
-    Ne[Γ |- n' : A] ->
     [Γ |- n : A] ->
     [Γ |- n' : A] ->
     [Γ |- n ~ n' : A] ->
     [Γ ||-<l> n : A | RA] × [Γ ||-<l> n ≅ n' : A| RA];
-  reify : forall a, [Γ ||-<l> a : A | RA] -> Nf[ Γ |- a : A];
 }.
 
 Lemma complete_reflect_simpl {l Γ A} (RA : [Γ ||-<l> A]) (c : complete RA) :
-  forall n, Ne[Γ |- n : A] -> [Γ |- n : A] -> [Γ |- n ~ n : A] -> [Γ ||-<l> n : A | RA].
+  forall n, [Γ |- n : A] -> [Γ |- n ~ n : A] -> [Γ ||-<l> n : A | RA].
 Proof.
 intros; eapply c.
-5: eassumption.
-all: assumption.
+all: eassumption.
 Qed.
 
 Lemma complete_var0 {l Γ A A'} (RA : [Γ ,, A ||-<l> A']) :
@@ -135,9 +112,6 @@ Proof.
   assert [Γ ,, A |- tRel 0 : A']
   by (eapply ty_conv; tea; escape; eapply (ty_var (wfc_wft EscRA) (in_here _ _))).
   eapply complete_reflect_simpl; tea.
-  - eapply tm_ne_conv; tea. 
-    2: now escape. 
-    now eapply tm_ne_rel.
   - eapply convneu_var; tea.
 Qed.
 
@@ -145,51 +119,27 @@ Qed.
 Lemma complete_U : forall l Γ A (RA : [Γ ||-U< l > A]), complete (LRU_ RA).
 Proof.
 intros l Γ A h0; split.
-- intros ? [].
-  eapply ty_nf_red, ty_nf_sort; gen_typing.
-- intros ?? ???? h; pose proof (lrefl h); pose proof (urefl h).
+- intros ???? h; pose proof (lrefl h); pose proof (urefl h).
   assert [Γ |- A ≅ U] by (destruct h0; gen_typing); split.
   2: unshelve econstructor.
   1-3: now apply neU.
-  + eapply RedTyRecBwd, neu. 2,3: try gen_typing.
-    eapply ty_ne_term, tm_ne_conv; tea; gen_typing.
+  + eapply RedTyRecBwd, neu. 1,2: try gen_typing.
   + cbn. gen_typing.
-  + eapply RedTyRecBwd; apply neu. 2, 3: gen_typing.
-    eapply ty_ne_term, tm_ne_conv; tea; gen_typing.
+  + eapply RedTyRecBwd; apply neu. 1,2: gen_typing.
   + eapply TyEqRecBwd. eapply neuEq. all: try gen_typing.
     all: eapply ty_ne_term, tm_ne_conv; tea; gen_typing.
-- intros a [a' Hr Ha].
-  assert ([Γ |-[ ta ] U ≅ A]).
-  { destruct h0; gen_typing. }
-  eapply tm_nf_conv; [| |eassumption].
-  + eapply tm_nf_red; [eapply tmr_wf_red|]; eassumption.
-  + now eapply escape, LRU_.
 Qed.
 
 Lemma complete_ne : forall l Γ A (RA : [Γ ||-ne A]), complete (LRne_ l RA).
 Proof.
 intros l Γ A h0; split.
-- intros ? [].
-  eapply ty_nf_red; [|now apply ty_ne_nf].
-  gen_typing.
 - destruct h0 as [B []]; intros ** ; assert ([Γ |- A ≅ B]) by gen_typing ; split.
   + exists n; cbn.
     * eapply redtmwf_refl ; gen_typing.
-    * now eapply tm_ne_conv.
     * eapply lrefl; eapply convneu_conv; eassumption.
   + exists n n'; cbn.
     1,2: eapply redtmwf_refl ; eapply ty_conv; gen_typing.
-    1,2: now eapply tm_ne_conv.
     gen_typing.
-- intros a [a' Hr Hne].
-  assert ([Γ |-[ ta ] neRedTy.ty h0 ≅ A]).
-  { destruct h0; simpl in *; symmetry.
-    eapply convty_exp; [now apply tyr_wf_red| |].
-    all: gen_typing. }
-  eapply tm_nf_conv; [| |eassumption].
-  + eapply tm_nf_red; [now apply tmr_wf_red|].
-    now apply tm_ne_nf.
-  + now eapply escape, LRne_ with (l := l).
 Qed.
 
 Lemma complete_Pi : forall l Γ A (RA : [Γ ||-Π< l > A]),
@@ -201,65 +151,29 @@ Lemma complete_Pi : forall l Γ A (RA : [Γ ||-Π< l > A]),
   complete (LRPi' RA).
 Proof.
 intros l Γ A ΠA0 ihdom ihcod; split.
-- intros B ΠB.
-  assert (tΓ : [|- Γ]) by (destruct ΠA0; gen_typing).
-  eapply ty_nf_red; [apply tyr_wf_red, ΠB|].
-  assert [PolyRed.shpRed ΠA0 wk_id tΓ | Γ ||- _ ≅ PiRedTyEq.dom ΠB].
-  1: erewrite <- wk_id_ren_on; eapply (PolyRedEq.shpRed ΠB).
-  eapply ty_nf_prod.
-  + now eapply ihdom.
-  + destruct ΠB as [dom cod ?? [domRed codRed]] ; cbn in *.
-    assert [|- Γ ,, dom]. 1:{
-      apply wfc_cons; tea.
-      now eapply escapeConv.
-    }
-    eapply ihcod.
-    replace cod with cod[tRel 0 .: @wk1 Γ dom >> tRel].
-    2: bsimpl ; rewrite scons_eta' ; now bsimpl.
-    eapply codRed.
-    Unshelve.  1: tea.
-    eapply complete_var0.
-      * eapply ihdom.
-      * symmetry; eapply escapeEq; erewrite <- wk1_ren_on.
-        unshelve eapply domRed. tea.
-      * now eapply escapeConv.
 - set (ΠA := ΠA0); destruct ΠA0 as [dom cod].
   simpl in ihdom, ihcod.
   assert [Γ |- A ≅ tProd dom cod] by gen_typing.
-  unshelve refine ( let funred : forall n, Ne[Γ |- n : A] -> [Γ |- n : A] -> [Γ |- n ~ n : A] -> [Γ ||-Π n : A | ΠA] := _ in _).
+  unshelve refine ( let funred : forall n, [Γ |- n : A] -> [Γ |- n ~ n : A] -> [Γ ||-Π n : A | ΠA] := _ in _).
   {
     intros. exists n; cbn.
     * eapply redtmwf_refl ; gen_typing.
-    * now eapply NeFun, tm_ne_whne.
-    * eapply tm_nf_conv; [| |eassumption].
-      + now eapply tm_ne_nf.
-      + gen_typing.
-    * gen_typing.
+    * now eapply NeFun, convneu_whne.
+    * eapply convtm_conv; [|eassumption].
+      now apply convtm_convneu.
     * intros; apply complete_reflect_simpl; [apply ihcod| |..].
-      { eapply neu_app_ren; try eassumption.
-        + gen_typing.
-        + now apply (ihdom _ ρ h). }
       1: escape ; now eapply ty_app_ren.
       eapply convneu_app_ren. 1,2: eassumption.
       eapply LREqTermRefl_ in ha.
       now escape.
     * intros. apply ihcod.
-      + eapply neu_app_ren; try eassumption.
-        -- gen_typing.
-        -- now apply (ihdom _ ρ h).
-      + eapply tm_ne_conv.
-        - eapply neu_app_ren; try eassumption.
-          -- gen_typing.
-          -- now apply (ihdom _ ρ h).
-        - now eapply escape, PolyRed.posRed.
-        - symmetry. unshelve eapply escapeEq, PolyRed.posExt; cycle 2; tea.
       + apply escapeTerm in ha; now eapply ty_app_ren.
       + escape; eapply ty_conv.
         1: now eapply ty_app_ren.
         symmetry; unshelve eapply escapeEq, PolyRed.posExt; cycle 2; tea.
       + apply escapeEqTerm in eq0; now eapply convneu_app_ren.
   }
-  intros ?????? h.
+  intros ???? h.
   pose proof (lrefl h); pose proof (urefl h).
   split. 1: now apply funred.
   unshelve econstructor.
@@ -267,23 +181,10 @@ intros l Γ A ΠA0 ihdom ihcod; split.
   all: cbn; clear funred.
   * gen_typing.
   * intros. apply ihcod; cbn.
-    + eapply neu_app_ren; try eassumption.
-      -- gen_typing.
-      -- now eapply (ihdom _ ρ).
-    + eapply neu_app_ren; try eassumption.
-      -- gen_typing.
-      -- now eapply (ihdom _ ρ).
     + apply escapeTerm in ha; now eapply ty_app_ren.
     + apply escapeTerm in ha; now eapply ty_app_ren.
     + eapply convneu_app_ren. 1,2: eassumption.
     eapply escapeEqTerm; eapply LREqTermRefl_; eassumption.
-- intros a [a' Hr Ha].
-  destruct ΠA0 as [dom codom]; simpl in *.
-  assert ([Γ |- tProd dom codom ≅ A ]) by gen_typing.
-  eapply tm_nf_conv; [| |eassumption].
-  * eapply tm_nf_red; [now apply tmr_wf_red|].
-    assumption.
-  * destruct red; gen_typing.
 Qed.
 
 Arguments ParamRedTy.outTy /.
@@ -300,38 +201,14 @@ Proof.
   assert [Γ |- A ≅ PA.(outTy)] by (destruct PA; cbn in *; gen_typing).
   assert [Γ |- PA.(outTy)] by (destruct PA; cbn in *; gen_typing). 
   split.
-  - intros B PB.
-    assert (tΓ : [|- Γ]) by (destruct PA; gen_typing).
-    eapply ty_nf_red; [apply tyr_wf_red, PB|].
-    assert [PolyRed.shpRed PA wk_id tΓ | Γ ||- _ ≅ PiRedTyEq.dom PB].
-    1: erewrite <- wk_id_ren_on; eapply (PolyRedEq.shpRed PB).
-    eapply ty_nf_sig.
-    + now eapply ihdom.
-    + destruct PB as [dom cod ?? [domRed codRed]] ; cbn in *.
-      assert [|- Γ ,, dom]. 1:{
-        apply wfc_cons; tea.
-        now eapply escapeConv.
-      }
-      eapply ihcod.
-      replace cod with cod[tRel 0 .: @wk1 Γ dom >> tRel].
-      2: bsimpl ; rewrite scons_eta' ; now bsimpl.
-      eapply codRed.
-      Unshelve.  1: tea.
-      eapply complete_var0.
-        * eapply ihdom.
-        * symmetry; eapply escapeEq; erewrite <- wk1_ren_on.
-          unshelve eapply domRed. tea.
-        * now eapply escapeConv.
   - 
-    unshelve refine ( let funred : forall n, Ne[Γ |- n : A] -> [Γ |- n : A] -> [Γ |- n ~ n : A] -> [Γ ||-Σ n : A | PA] := _ in _).
+    unshelve refine ( let funred : forall n, [Γ |- n : A] -> [Γ |- n ~ n : A] -> [Γ ||-Σ n : A | PA] := _ in _).
     1:{
       intros n **.
       assert (hfst : forall Δ (ρ : Δ ≤ Γ) (h : [ |- Δ]), [PolyRedPack.shpRed PA ρ h | Δ ||- tFst n⟨ρ⟩ : _]).
       1:{
         intros; eapply complete_reflect_simpl.
         * eapply ihdom.
-        * rewrite wk_fst; eapply tm_ne_wk; tea.
-          eapply tm_ne_fst; now eapply tm_ne_conv. 
         * rewrite wk_fst; eapply ty_wk; tea.
           eapply ty_fst; now eapply ty_conv.
         * rewrite wk_fst; eapply convneu_wk; tea.
@@ -339,14 +216,12 @@ Proof.
       }
       exists n hfst.
       + eapply redtmwf_refl; now eapply ty_conv.
-      + constructor; now eapply tm_ne_whne.
-      + eapply tm_ne_nf; now eapply tm_ne_conv.
+      + constructor; now eapply convneu_whne.
       + eapply convtm_convneu; now eapply convneu_conv.
       + intros; irrelevanceRefl.
         eapply complete_reflect_simpl; [unshelve eapply ihcod|..]; tea.
         1: eapply hfst.
         all: rewrite wk_fst; rewrite <- subst_ren_subst_mixed; rewrite wk_snd.
-        * eapply tm_ne_wk; tea; eapply tm_ne_snd; now eapply tm_ne_conv.
         * eapply ty_wk; tea; eapply ty_snd; now eapply ty_conv.
         * eapply convneu_wk; tea; eapply convneu_snd; now eapply convneu_conv.
     }
@@ -359,22 +234,16 @@ Proof.
       [PolyRedPack.shpRed PA ρ h | Δ ||- tFst n⟨ρ⟩ ≅ tFst n'⟨ρ⟩ : (ParamRedTyPack.dom PA)⟨ρ⟩]).
     1:{
       intros; cbn; eapply ihdom.
-      * rewrite wk_fst; eapply tm_ne_wk; tea.
-        eapply tm_ne_fst; now eapply tm_ne_conv. 
-      * rewrite wk_fst; eapply tm_ne_wk; tea.
-        eapply tm_ne_fst; now eapply tm_ne_conv. 
       * rewrite wk_fst; eapply ty_wk; tea.
         eapply ty_fst; now eapply ty_conv.
       * rewrite wk_fst; eapply ty_wk; tea.
-        eapply ty_fst; now eapply ty_conv.
+        eapply ty_fst; now eapply ty_conv. 
       * do 2 rewrite wk_fst; eapply convneu_wk; tea.
         eapply convneu_fst; now eapply convneu_conv.
     }
-    assert (hcod : forall (Δ : context) (ρ : Δ ≤ Γ) (h : [ |-[ ta ] Δ]), [Δ |- (ParamRedTy.cod PA)[tFst n⟨ρ⟩ .: ρ >> tRel] ]).
-    1: intros; eapply escape; unshelve eapply (PolyRed.posRed PA); tea; eapply Rn.
     assert (forall (Δ : context) (ρ : Δ ≤ Γ) (h : [ |-[ ta ] Δ]),
       [Δ |- (ParamRedTy.cod PA)[tFst n⟨ρ⟩ .: ρ >> tRel] ≅ (ParamRedTy.cod PA)[tFst n'⟨ρ⟩ .: ρ >> tRel]]).
-    1:{
+    {
       intros; eapply escapeEq; unshelve eapply (PolyRed.posExt PA); tea.
       + eapply Rn.
       + eapply Rn'.
@@ -385,71 +254,39 @@ Proof.
     + apply Rnn'.
     + intros; cbn; eapply ihcod.
       all: rewrite wk_fst; rewrite !wk_snd.
-      2: eapply tm_ne_conv; [| apply hcod; tea |now symmetry]; rewrite wk_fst.
-      4: eapply ty_conv; [|now symmetry]; rewrite wk_fst.
+      2: eapply ty_conv; [|now symmetry]; rewrite wk_fst.
       all: rewrite <- subst_ren_subst_mixed.
-      * eapply tm_ne_wk; tea; eapply tm_ne_snd; now eapply tm_ne_conv.
-      * eapply tm_ne_wk; tea; eapply tm_ne_snd ; now eapply tm_ne_conv.
       * eapply ty_wk; tea; eapply ty_snd; now eapply ty_conv.
       * eapply ty_wk; tea; eapply ty_snd; now eapply ty_conv.
       * eapply convneu_wk; tea; eapply convneu_snd; now eapply convneu_conv.
-  - intros a [].
-    eapply tm_nf_conv; [gen_typing| destruct PA; gen_typing |now symmetry].
 Qed.
 
 Lemma complete_Nat {l Γ A} (NA : [Γ ||-Nat A]) : complete (LRNat_ l NA).
 Proof.
   split.
-  - intros ? [].
-    eapply ty_nf_red, ty_nf_nat; gen_typing.
   - intros. 
     assert [Γ |- A ≅ tNat] by (destruct NA; gen_typing). 
     assert [Γ |- n : tNat] by now eapply ty_conv.
     split; econstructor.
     1,4,5: eapply redtmwf_refl; tea; now eapply ty_conv.
     2,4: do 2 constructor; tea.
-    1,7: eapply convtm_convneu.
-    1,4: eapply lrefl.
-    4-6: now (eapply tm_ne_conv; gen_typing).
-    all: eapply convneu_conv; tea.
-  - simpl in *.
-    assert [Γ |- tNat ≅ A] by (destruct NA; gen_typing).
-    assert [Γ |- A] by now (destruct NA; gen_typing).
-    intros a Ha; eapply tm_nf_conv; [|eassumption|eassumption]; revert a Ha.
-    let T := match goal with |- ?P => P end in
-    enough (IH : T × (forall (a : term) (n : NatProp NA a), Nf[ Γ |-[ ta ] a : tNat])); [apply IH|].
-    apply NatRedInduction.
-    + intros.
-      eapply tm_nf_red; [now apply tmr_wf_red|eassumption].
-    + eapply tm_nf_zero; gen_typing.
-    + intros; now eapply tm_nf_succ.
-    + intros ne []. apply tm_ne_nf. assumption.
+    1,4: eapply convtm_convneu.
+    all: eapply convneu_conv; [|eassumption].
+    all: first [assumption|now eapply lrefl].
 Qed.
 
 Lemma complete_Empty {l Γ A} (NA : [Γ ||-Empty A]) : complete (LREmpty_ l NA).
 Proof.
   split.
-  - intros ? [].
-    eapply ty_nf_red, ty_nf_empty; gen_typing.
   - intros. 
     assert [Γ |- A ≅ tEmpty] by (destruct NA; gen_typing). 
     assert [Γ |- n : tEmpty] by now eapply ty_conv.
     split; econstructor.
     1,4,5: eapply redtmwf_refl; tea; now eapply ty_conv.
     2,4: do 2 constructor; tea.
-    1,7: eapply convtm_convneu.
-    1,4: eapply lrefl.
-    4-6: now (eapply tm_ne_conv; gen_typing).
-    all: eapply convneu_conv; tea.
-  - simpl in *.
-    assert [Γ |- tEmpty ≅ A] by (destruct NA; gen_typing).
-    intros a Ha; eapply tm_nf_conv; [| |eassumption].
-    + destruct Ha.
-      destruct prop.
-      destruct r.
-      eapply tm_nf_red. exact red.
-      now apply tm_ne_nf.
-    + destruct NA as [[]]; gen_typing.
+    1,4: eapply convtm_convneu.
+    all: eapply convneu_conv; [|eassumption].
+    all: try first [assumption|now eapply lrefl].
 Qed.
 
 Lemma completeness {l Γ A} (RA : [Γ ||-<l> A]) : complete RA.
@@ -464,7 +301,6 @@ revert l Γ A RA; eapply LR_rect_TyUr; cbn; intros.
 Qed.
 
 Lemma neuTerm {l Γ A} (RA : [Γ ||-<l> A]) {n} :
-  Ne[Γ |- n : A] ->
   [Γ |- n : A] ->
   [Γ |- n ~ n : A] ->
   [Γ ||-<l> n : A | RA].
@@ -473,8 +309,6 @@ Proof.
 Qed.
 
 Lemma neuTermEq {l Γ A} (RA : [Γ ||-<l> A]) {n n'} :
-  Ne[Γ |- n : A] ->
-  Ne[Γ |- n' : A] ->
   [Γ |- n : A] ->
   [Γ |- n' : A] ->
   [Γ |- n ~ n' : A] ->
@@ -501,18 +335,6 @@ Proof.
   rewrite eq.
   unshelve eapply escapeEq; tea.
   eapply LRTyEqRefl_.
-Qed.
-
-Lemma reifyTerm {l Γ A} (RA : [Γ ||-<l> A]) {t} : [Γ ||-<l> t : A | RA] -> Nf[Γ |- t : A].
-Proof.
-intros; now eapply completeness.
-Qed.
-
-Lemma reifyType {l Γ A} (RA : [Γ ||-<l> A]) : Nf[Γ |- A].
-Proof.
-  unshelve eapply reifyTyConv; tea.
-  1: now eapply completeness.
-  apply LRTyEqRefl_.
 Qed.
 
 End Neutral.
