theories/LogicalRelation/Induction.v
@@ -181,7 +181,7 @@ Section Inversions.
     `{!WfContext ta} `{!WfType ta} `{!Typing ta}
     `{!ConvType ta} `{!ConvTerm ta} `{!ConvNeuConv ta}
     `{!RedType ta} `{!TypeNf ta} `{!TypeNe ta} `{!RedTerm ta} `{!TermNf ta} `{!TermNe ta} `{!RedTypeProperties}
-    `{!TypeNeProperties}.
+    `{!TypeNeProperties} `{!ConvNeuProperties}.
 
 
   Lemma invLR {Γ l A A'} (lr : [Γ ||-<l> A]) (r : [A ⇒* A']) (w : isType A') :
@@ -210,7 +210,7 @@ Section Inversions.
     - intros * ? A' red whA.
       enough ({w' & whA = NeType w'}) as [? ->] by easy.
       destruct neA as [A'' redA neA''].
-      apply ty_ne_whne in neA''.
+      apply convneu_whne in neA''.
       assert (A' = A'') as <-.
       + eapply whred_det.
         1-3: gen_typing.
